\documentclass[12pt]{article}
\usepackage{geometry}
\usepackage{enumitem}
\usepackage{graphicx}
\usepackage{amsmath}
\usepackage{mathtools}
\usepackage{xcolor}
\usepackage{cancel}
\usepackage{titlesec}
\newcommand{\note}[1]{{\color{red} #1 }}
\newcommand{\fignote}[1]{{\color{blue} #1 }}
\renewcommand{\v}[1]{\boldsymbol{ #1 }}
\renewcommand{\bar}[1]{\overline{ #1 }}
\newcommand{\vh}[1]{\hat{\boldsymbol{ #1 }}}
\newcommand{\dd}[2]{\frac{\partial #1}{\partial #2}}
\newcommand{\cE}{\mathcal{E}}
\newcommand{\ebar}{\overline{e}}
\newcommand{\gammabar}{\overline{\gamma}}
\newcommand{\thetabar}{\overline{\theta}}
\newcommand{\edisk}{e_d}
\DeclarePairedDelimiter{\abs}{|}{|}
\DeclarePairedDelimiter{\br}{[}{]}
\DeclarePairedDelimiter{\p}{(}{)}
\DeclarePairedDelimiter{\we}{\langle}{\rangle}

\title{4 dof Hamiltonian differential equations}

\begin{document}
\maketitle
\section{Hamiltonian \& Scaling}
Let $m_1$ denote the inner planet and $m_2$ denote the outer planet.
\begin{equation}
H=-\frac{G M m_{1}}{2 a_{1}}-\frac{G M m_{2}}{2 a_{2}}
-\frac{G m_{1} m_{2}}{a_{2}}  \left(f_{1} e_{1} \cos \theta_{1} 
+f_{2} e_{2} \cos \theta_{2}\right)
\end{equation}

\begin{align*}
  \theta &= (j+1)\lambda_2 - j\lambda_1\\
  \theta_1 &= (j+1)\lambda_2 - j\lambda_1+\gamma_1\\
  \theta_2 &= (j+1)\lambda_2 - j\lambda_1+\gamma_2\\
  q &= \frac{m_1}{m_2}\\
  a_0&= a_{2,\rm init} \\
  H_0 &= \frac{GMm_2}{a_0}\\
  \omega_0 &= n_{2,\rm init} = \sqrt{\frac{GM}{a_0^3}}\\
  \Lambda_0 &= m_2\sqrt{GMa_0}
\end{align*}

\begin{align*}
  \alpha_1 &= \frac{a_1}{a_0}\\
  \alpha_2 &= \frac{a_2}{a_0}\\
  \Lambda_1 &= q\sqrt{\alpha_1}\\
  \Lambda_2 &= \sqrt{\alpha_2}\\
  x_1 &= \Gamma_1\cos(\gamma_1)\\ 
  y_1 &= \Gamma_1\sin(\gamma_1)\\ 
  x_2 &= \Gamma_2\cos(\gamma_2)\\ 
  y_2 &= \Gamma_2\sin(\gamma_2)\\ 
\end{align*}


\section{Resonant Equations of Motion}
\begin{equation}
  \label{eq:2}
  \overline{H} = -\frac{q^3}{2\Lambda_1^2} -\frac{1}{2\Lambda_2^2} - \frac{q\mu_2}{\Lambda_2^2}\p*{ f_1 \sqrt{\frac{2\Gamma_1}{\Lambda_1}}\cos\theta_1 + f_2\sqrt{\frac{2\Gamma_2}{\Lambda_2}}\cos\theta_2}
\end{equation}
\note{Note: $f_1 = -A, f_2 = -B$}

\textbf{Integration variables:} $(\theta, \Lambda_1, \Lambda_2, x_1, y_1, x_2, y_2)$


\begin{equation}
\dot{\lambda}_{1}=\frac{1}{\alpha_1^{3 / 2}}+\frac{\mu_{2} f_{1} e_{1}}{2 \alpha_{2} \alpha_{1}^{1 / 2}} \cos \theta_{1}
\end{equation}

\begin{equation}
\dot{\lambda}_{2}=\frac{1}{\alpha_{2}^{3 / 2}}+\frac{q \mu_{2}}{\alpha_{2}^{3 / 2}}\left(
2 f_{1} e_{1} \cos \theta_{1}
+\frac{5}{2} f_{2} e_{2} \cos \theta_{2}
\right)
\end{equation}

\begin{equation}
\dot{\Lambda}_{1}=\frac{jq \mu_{2}}{\alpha_{2}} \left(f_{1} e_{1} \sin \theta_{1}+f_{2} e_{2} \sin \theta_{2}\right)
\end{equation}

\begin{equation}
\dot{\Lambda}_2=-\frac{(j+1)q \mu_{2}}{\alpha_{2}}\left(f_{1} e_{1} \sin \theta_{1}+f_{2} e_{2} \sin \theta_{2}\right)
\end{equation}

\begin{equation}
\dot{\gamma}_{1}=\frac{- \mu_{2}}{\sqrt\alpha_{1} \alpha_{2} e_{1}} f_{1} \cos \theta_{1}
\end{equation}

\begin{equation}
\dot{\gamma}_{2}=-\frac{q \mu_{2}}{\alpha_{2}^{3/2} e_{2}} f_{2} \cos \theta_{2} 
\end{equation}
\begin{equation}
\dot{\Gamma}_{1}=-\frac{q \mu_{2}}{\alpha_{2}} f_{1} e_{1} \sin \theta_{1}
\end{equation}
\begin{equation}
\dot{\Gamma}_{2}=-\frac{q \mu_{2}}{\alpha_{2}} f_{2} e_{2} \sin \theta_{2}
\end{equation}
\begin{equation}
\dot{x}_{1} = \dot{\Gamma}_{1}\cos(\gamma_1) - \Gamma_1\sin(\gamma_1)\dot{\gamma}_{1}
\end{equation}
\begin{equation}
\dot{y}_{1} = \dot{\Gamma}_{1}\sin(\gamma_1) + \Gamma_1\cos(\gamma_1)\dot{\gamma}_{1}
\end{equation}
\begin{equation}
\dot{x}_{2} = \dot{\Gamma}_{2}\cos(\gamma_2) - \Gamma_2\sin(\gamma_2)\dot{\gamma}_{2}
\end{equation}
\begin{equation}
\dot{y}_{2} = \dot{\Gamma}_{2}\sin(\gamma_2) + \Gamma_2\cos(\gamma_2)\dot{\gamma}_{2}
\end{equation}


\section{Secular Equations of Motion}

\begin{equation}
  \overline H_{\rm sec}
  = -\frac{q\mu_2}{\Lambda_2^2}
  \p*{
    \frac{2C\Gamma_1}{\Lambda_1}
    +\frac{2C\Gamma_2}{\Lambda_2}
    +D\sqrt{\frac{2\Gamma_1}{\Lambda_1}}
    \sqrt{\frac{2\Gamma_2}{\Lambda_2}}
    \cos(\gamma_1-\gamma_2)
    }
\end{equation}

\begin{equation}
\dot{\lambda}_{1}=\frac{ \mu_{2}}{\alpha_{2} \sqrt{\alpha_{1}}}\left(C e_{1}^{2}+\frac{D e_{1} e_{2}}{2} \cos \left(\gamma_{1}-\gamma_{2}\right)\right) 
\end{equation}
\begin{equation}
\dot{\lambda}_{2}=\frac{q \mu_{2}}{\alpha_{2}^{3 / 2}}\left(2 C e_{1}^{2}+3 C e_{2}^{2}+\frac{5}{2} De_{1}e_2 \cos \left(\gamma_1-\gamma_2\right)\right)
\end{equation}
\begin{equation}
\dot{\Gamma}_{1}=\frac{q \mu_{2} D e_{1} e_{2}}{\alpha_{2}} \sin \left(\gamma_{2}-\gamma_{1}\right)
\end{equation}
\begin{equation}
\dot{\Gamma}_{2}=\frac{q \mu_{2} D e_{1} e_{2}}{\alpha_{2}} \sin \left(\gamma_{1}-\gamma_{2}\right) 
\end{equation}
\begin{equation}
\dot{\gamma}_{1}=-\frac{ \mu_{2}}{\alpha_{2} \sqrt{\alpha_{1}}}\left(2 C+D \frac{e_{2}}{e_{1}}\right) 
\end{equation}
\begin{equation}
\dot{\gamma}_{2}=-\frac{q \mu_{2}}{\alpha_{2}^{3 / 2}}\left(2 C+D \frac{e_{1}}{e_{2}}\right)
\end{equation}
\section{Dissipation}
\textbf{Parameters:} $(T_{m,2}, T_{e,1}, T_{e,2})$; i.e. $T_{m,1} = \infty$; $T_e>0$; $T_m<0$
\begin{equation}
  \dot{\Lambda}_{1,\rm{dis}} = -\frac{\Lambda_1}{2}\p*{\frac{4\Gamma_1}{\Lambda_1T_{e,1}}}
\end{equation}
\begin{equation}
  \dot{\Lambda}_{2,\rm{dis}} = \frac{\Lambda_1}{2}\p*{\frac{1}{T_{m,2}}-\frac{4\Gamma_2}{\Lambda_2T_{e,2}}}
\end{equation}
\begin{equation}
 \dot x_{1,\rm{dis}} = -\sqrt \Gamma_2\cos(\gamma_1) \p*{\frac{1}{T_{e,1}} + \frac{\Gamma_1}{T_{e,1}\Lambda_1}}
\end{equation}
\begin{equation}
 \dot y_{1,\rm{dis}} = -\sqrt \Gamma_2\sin(\gamma_1) \p*{\frac{1}{T_{e,1}} + \frac{\Gamma_1}{T_{e,1}\Lambda_1}}
\end{equation}
\begin{equation}
 \dot x_{2,\rm{dis}} = \sqrt \Gamma_2\cos(\gamma_2) \p*{-\frac{1}{T_{e,2}} +\frac14\p*{\frac{1}{T_{m,2}}- \frac{4\Gamma_2}{T_{e,2}\Lambda_2}}}
\end{equation}
\begin{equation}
 \dot y_{2,\rm{dis}} = \sqrt \Gamma_2\sin(\gamma_2) \p*{-\frac{1}{T_{e,2}} +\frac14\p*{\frac{1}{T_{m,2}}- \frac{4\Gamma_2}{T_{e,2}\Lambda_2}}}
\end{equation}
\section{Equilibrium}
\begin{equation}
  \dot e_1 = \frac{\mu_2}{\alpha_2} [f_1\sin(\theta_1) - De_2 \sin(\gamma_2-\gamma_1)]
\end{equation}

\begin{equation}
  \dot e_2 = \frac{q\mu_2}{\alpha_2} [f_2\sin(\theta_2) - De_1 \sin(\gamma_1-\gamma_2)]
\end{equation}

\begin{equation}
  \dot\varpi_1-\dot\varpi_2 = \frac{\mu_2}{\alpha_2}\p*{ \frac{f_1\cos\theta_1}{\alpha_1^{1/2} e_1} - \frac{qf_2\cos\theta_2}{\alpha_2^{1/2}e_2}
    + \frac{2C}{\alpha_1^{1/2}} + \frac{De_2}{\alpha_1^{1/2} e_1} - \frac{2qC}{\alpha_2^{1/2}} - \frac{qDe_1}{ \alpha_2^{1/2}e_2}}
\end{equation}

\begin{align*}
  \dot\eta &= \frac{q\alpha_0^{1/2}}{j(q\alpha_0^{-1}+1)}\br*{ \frac{1}{T_{m2}} - \frac{1}{T_{m1}}
      + \frac{2e_1^2}{T_{e1}}- \frac{2e_2^2}{T_{e2}}}
    - q\alpha_0^{1/2}\frac{2e_1^2}{T_{e1}} - \frac{2e_2^2}{T_{e2}}\\
    &\quad+ \cancel{\underbrace{\p*{q \frac{\mu_2\sin(\varpi_1 -\varpi_2)}{\alpha_2^{3/2}}De_1e_2
      + q\frac{\mu_2\sin(\varpi_2 -\varpi_1)}{\alpha_2^{3/2}}De_1e_2}}}_{{\color{red}\text{secular contributions}}}
\end{align*}
\end{document}